fix SUFCMA initialisation, push signedDH forward a bit

signedDH/easycrypt/SignedDH.ec
@@ -123,6 +123,185 @@ module SignedDH (S : SigScheme) (H : RO) : UATPaKE = {
   }
 }.
 
+module B1 (S : SigScheme) (A : Adv_UATPaKE_RO) (O : CMA_Oracles) = {
+  var b_ror : bool
+
+  var forgery : (int * (pdh * pdh) * sig) option
+
+  var n : int
+  var m : int
+  
+  var p_map : (int, int) fmap
+  var i_map : (int, pdh) fmap
+  var h_map : (pdh * pdh * pdh, sskey) fmap
+  var r_map : (int option * int, (pdh * sig) fset) fmap
+
+  var pk_map : (int, pkey) fmap
+  var c_map : (int, client_state) fmap
+  
+  var q : int fset
+  var ich : int fset
+  var rch : int fset
+  var xp : int fset
+  var cr : int fset
+  
+  module Oracles = {
+    proc gen(): pkey = {
+      var pk;
+
+      pk <@ O.gen();
+      if (has (fun i pk_i=> pk_i = pk /\ p_map.[i] = None) pk_map) {
+        pk <- witness;
+      } else {
+        m <- m + 1;
+        pk_map.[m] <- pk;
+      }
+      
+      return pk;
+    }
+
+    proc corrupt(j: int): skey option = {
+      var r <- None;
+
+      if (0 < j <= m) {
+        r <@ O.corrupt(j);
+        cr <- cr `|` fset1 j;
+      }
+      return r;
+    }
+
+    proc expose(i) = {
+      var r <- None;
+
+      if (0 < i <= n /\ i \notin ich) {
+        xp <- xp `|` fset1 i;
+        r <- c_map.[i];
+      }
+      return r;
+    }
+
+    proc init(pk: pkey): pdh = {
+      var st, jo, c, x;
+
+      n <- n + 1;
+      x <$ dsk;
+      c <- g ^ x;
+      st <- {| pk = pk; epk = c; esk = x; |};
+      c_map.[n] <- st;
+      jo <- find (fun _ pk_j=> pk_j = pk) pk_map;
+      if (jo is Some j) {
+        p_map.[n] <- j;
+        i_map.[n] <- c;
+      }
+      return c;
+    }
+
+    proc respond(j: int, c: pdh, ch: bool): (sskey * (pdh * sig)) option = {
+      var k, c', io, h, y, sig;
+      var r <- None;
+
+      if (0 < j <= m) {
+        y <$ dsk;
+        h <- g ^ y;
+        sig <@ O.sign(j, (c, h));
+        k <@ RO.get(c, h, c ^ y);
+        c' <- (h, oget sig);
+        io <- find (fun i j' => j' = j /\ i_map.[i] = Some c) p_map;
+        if (io is Some i) {
+          r_map.[Some j, i] <- (odflt fset0 r_map.[Some j, i]) `|` fset1 c';
+          if (ch /\ i \notin xp) {
+            if (b_ror) { k <$ dssk; }
+            ich <- ich `|` fset1 i;
+          }
+        }
+        r <- Some (k, c');
+      }
+      return r;
+    }
+
+    proc receive(i: int, c: pdh * sig, ch: bool): sskey option = {
+      var st_i, k, h, sig, b;
+      var ko <- None;
+
+      if (0 < i <= n /\ i \notin q) {
+        st_i <- oget c_map.[i];
+        q <- q `|` fset1 i;
+        
+        if (c \notin odflt fset0 r_map.[p_map.[i], i]) {
+          (h, sig) <- c;
+          b <@ S.verify(st_i.`pk, (st_i.`epk, h), sig);
+          if (b) {
+            k <@ RO.get(st_i.`epk, h, h ^ st_i.`esk);
+            ko <- Some k;
+          }
+          if (   ch
+              /\ i \notin xp
+              /\ p_map.[i] <> None /\ 0 < oget p_map.[i] <= m /\ oget p_map.[i] \notin cr
+              /\ ko <> None) {
+            if (forgery <> None) {
+              forgery <- Some (oget p_map.[i], (st_i.`epk, h), sig);
+            }
+            if (b_ror) { k <$ dssk; ko <- Some k; }
+            ich <- ich `|` fset1 i;
+          }
+        }
+      }
+      return ko;
+    }
+
+    proc h = RO.get
+  }
+
+  proc forge() = {
+    var b';
+
+    RO.init();
+
+    forgery <- None;
+
+    m <- 0;
+    n <- 0;
+
+    q <- fset0;
+    ich <- fset0;
+    rch <- fset0;
+    xp <- fset0;
+    cr <- fset0;
+
+    p_map <- empty;
+    i_map <- empty;
+    r_map <- empty;
+
+    pk_map <- empty;
+    c_map <- empty;
+
+    h_map <- empty;
+
+    b' <@ A(Oracles).distinguish();
+    return oget forgery;
+  }
+}.
+
+module B1_0 (S : SigScheme) (A : Adv_UATPaKE_RO) (O : CMA_Oracles) = {
+  proc forge() = {
+    var f;
+
+    B1.b_ror <- false;
+    f <@ B1(S, A, O).forge();
+    return f;
+  }
+}.
+
+module B1_1 (S : SigScheme) (A : Adv_UATPaKE_RO) (O : CMA_Oracles) = {
+  proc forge() = {
+    var f;
+
+    B1.b_ror <- true;
+    f <@ B1(S, A, O).forge();
+    return f;
+  }
+}.
+
 module B2 (S : SigScheme) (A : Adv_UATPaKE_RO) (O : St_CDH_Oracles) = {
   include var Exp_b(SignedDH(S), RO, A) [-run]
 
@@ -198,11 +377,11 @@ module B2 (S : SigScheme) (A : Adv_UATPaKE_RO) (O : St_CDH_Oracles) = {
     }
 
     proc init(pk: pkey): pdh = {
-      var st, jo, c, epk;
+      var st, jo, c;
 
       n <- n + 1;
-      epk <@ O.gen_1();
-      st <- {| pk = pk; epk = epk; esk = witness; |};
+      c <@ O.gen_1();
+      st <- {| pk = pk; epk = c; esk = witness; |};
       c_map.[n] <- st;
       jo <- find (fun _ pk_j=> pk_j = pk) pk_map;
       if (jo is Some j) {
@@ -217,6 +396,7 @@ module B2 (S : SigScheme) (A : Adv_UATPaKE_RO) (O : St_CDH_Oracles) = {
       var r <- None;
 
       if (0 < j <= m) {
+        y <- witness; (* silence a warning: all paths that use y define it first *)
         if (has (fun i j' => j' = j /\ i_map.[i] = Some c) p_map) {
           h <@ O.gen_2();
         } else {
@@ -306,8 +486,8 @@ module B2 (S : SigScheme) (A : Adv_UATPaKE_RO) (O : St_CDH_Oracles) = {
 }.
 
 section.
-declare module S <: SigScheme { -Exp_b, -RO }.
-declare module A <: Adv_UATPaKE_RO { -Exp_b, -RO, -S }.
+declare module S <: SigScheme { -Exp_b, -SUFCMA, -RO, -B1, -B2 }.
+declare module A <: Adv_UATPaKE_RO { -Exp_b, -SUFCMA, -RO, -B1, -B2, -S }.
 
 local module Game0_b = {
   include var Exp_b(SignedDH(S), RO, A) [-run]
@@ -475,7 +655,6 @@ call (: ={glob Exp_b(SignedDH(S), RO)}); last first.
   by sim.
 qed.
 
-
 local module Game1_b = {
   include var Exp_b(SignedDH(S), RO, A) [-run]
 
@@ -483,6 +662,8 @@ local module Game1_b = {
   var bad_2: bool
 
   module Oracles = {
+    include Game0_b.Oracles [-gen]
+
     proc gen(): pkey = {
       var pk, sk;
   
@@ -504,30 +685,85 @@ local module Game1_b = {
       
       return pk;
     }
-  
+  }
+
+  proc run(b) = {
+    var b';
+
+    RO.init();
+
+    b_ror <- b;
+
+    m <- 0;
+    n <- 0;
+
+    q <- fset0;
+    ich <- fset0;
+    rch <- fset0;
+    xp <- fset0;
+    cr <- fset0;
+
+    p_map <- empty;
+    i_map <- empty;
+    r_map <- empty;
+
+    pk_map <- empty;
+    sk_map <- empty;
+    c_map <- empty;
+
+    bad_1 <- false;
+    bad_2 <- false;
+
+    b' <@ A(Oracles).distinguish();
+    return b';
+  }
+}.
+
+local module Game2_b = {
+  include var Exp_b(SignedDH(S), RO, A) [-run]
+  include var Game1_b [-run]
+
+  module Oracles = {
+    proc gen(): pkey = {
+      var pk, sk;
+
+      (pk, sk) <@ S.keygen();
+      if (has (fun i st=> st.`pk = pk /\ p_map.[i] = None) c_map) {
+        bad_1 <- true;
+        (* Here, we don't stop; we just don't actually register the key and move on *)
+        pk <- witness;
+      } else {
+        m <- m + 1;
+        pk_map.[m] <- pk;
+        sk_map.[m] <- sk;
+      }
+      
+      return pk;
+    }
+
     proc corrupt(j: int): skey option = {
       var r <- None;
-  
+
       if (0 < j <= m) {
         r <- sk_map.[j];
         cr <- cr `|` fset1 j;
       }
       return r;
     }
-  
+
     proc expose(i) = {
       var r <- None;
-  
+
       if (0 < i <= n /\ i \notin ich) {
         xp <- xp `|` fset1 i;
         r <- c_map.[i];
       }
       return r;
     }
-  
+
     proc init(pk: pkey): pdh = {
       var st, jo, c, x;
-  
+
       n <- n + 1;
       x <$ dsk;
       c <- g ^ x;
@@ -540,11 +776,11 @@ local module Game1_b = {
       }
       return c;
     }
-  
+
     proc respond(j: int, c: pdh, ch: bool): (sskey * (pdh * sig)) option = {
       var k, c', io, sk_j, h, y, sig;
       var r <- None;
-  
+
       if (0 < j <= m) {
         sk_j <- oget sk_map.[j];
         y <$ dsk;
@@ -567,11 +803,11 @@ local module Game1_b = {
       }
       return r;
     }
-  
+
     proc receive(i: int, c: pdh * sig, ch: bool): sskey option = {
       var st_i, k, h, sig, b;
       var ko <- None;
-  
+
       if (0 < i <= n /\ i \notin q) {
         st_i <- oget c_map.[i];
         q <- q `|` fset1 i;
@@ -587,14 +823,15 @@ local module Game1_b = {
               /\ i \notin xp
               /\ p_map.[i] <> None /\ 0 < oget p_map.[i] <= m /\ oget p_map.[i] \notin cr
               /\ ko <> None) {
-            if (b_ror) { k <$ dssk; ko <- Some k; }
+            bad_2 <- true;
+            ko <- None;
             ich <- ich `|` fset1 i;
           }
         }
       }
       return ko;
     }
-  
+
     proc h = RO.get
   }
 
@@ -629,6 +866,24 @@ local module Game1_b = {
     return b';
   }
 }.
+
+(** We now successively state and prove claims about consecutive games
+    in the sequence. We sometimes introduce intermediate modules as
+    proof artefacts to enable formal reasoning.
+**)
+
+(** Hop 1: Game 0 and Game 1 are equivalent (regardless of the value
+    of the challenge bit) unless (and until) the gen oracle outputs a
+    public key that was already used by the adversary.
+
+    This happens with a probability bounded by the guessing entropy of
+    the distribution induced on public keys by key generation.
+**)
+local lemma Hop1 (b : bool) &m:
+  `|Pr[Game0_b.run(b) @ &m: res] - Pr[Game1_b.run(b) @ &m: res]|
+  <= Pr[Game1_b.run(b) @ &m: Game1_b.bad_1].
+(* This aborts the proof - we simply use the statement as a section heading. *)
+abort.
 
 (* In order to get the absolute values in, we need to make sure that
    we can express the bad event on the left of the hop. While we do
@@ -808,158 +1063,78 @@ call (: Game1_b.bad_1 (* the bad event *)
 by inline; auto=> /> /#.
 qed.
 
-local module Game2_b = {
-  include var Exp_b(SignedDH(S), RO, A) [-run]
-  include var Game1_b [-run]
-
-  module Oracles = {
-    proc gen(): pkey = {
-      var pk, sk;
-
-      (pk, sk) <@ S.keygen();
-      if (has (fun i st=> st.`pk = pk /\ p_map.[i] = None) c_map) {
-        bad_1 <- true;
-        (* Here, we don't stop; we just don't actually register the key and move on *)
-        pk <- witness;
-      } else {
-        m <- m + 1;
-        pk_map.[m] <- pk;
-        sk_map.[m] <- sk;
-      }
-      
-      return pk;
-    }
-
-    proc corrupt(j: int): skey option = {
-      var r <- None;
-
-      if (0 < j <= m) {
-        r <- sk_map.[j];
-        cr <- cr `|` fset1 j;
-      }
-      return r;
-    }
-
-    proc expose(i) = {
-      var r <- None;
-
-      if (0 < i <= n /\ i \notin ich) {
-        xp <- xp `|` fset1 i;
-        r <- c_map.[i];
-      }
-      return r;
-    }
-
-    proc init(pk: pkey): pdh = {
-      var st, jo, c, x;
-
-      n <- n + 1;
-      x <$ dsk;
-      c <- g ^ x;
-      st <- {| pk = pk; epk = c; esk = x |};
-      c_map.[n] <- st;
-      jo <- find (fun _ pk_j=> pk_j = pk) pk_map;
-      if (jo is Some j) {
-        p_map.[n] <- j;
-        i_map.[n] <- c;
-      }
-      return c;
-    }
-
-    proc respond(j: int, c: pdh, ch: bool): (sskey * (pdh * sig)) option = {
-      var k, c', io, sk_j, h, y, sig;
-      var r <- None;
-
-      if (0 < j <= m) {
-        sk_j <- oget sk_map.[j];
-        y <$ dsk;
-        h <- g ^ y;
-        sig <@ S.sign(sk_j, (c, h));
-        c' <- (h, sig);
-        k <@ RO.get(c, h, c ^ y);
-        io <- find (fun i _=> p_map.[i] = Some j /\ i_map.[i] = Some c) c_map;
-        if (io is Some i) {
-          (*** Instead of initialising all of r_map to output the
-          empty set, we read undefined entries as the empty set
-          here. ***)
-          r_map.[Some j, i] <- (odflt fset0 r_map.[Some j, i]) `|` fset1 c';
-          if (ch /\ i \notin xp) {
-            if (b_ror) { k <$ dssk; }
-            ich <- ich `|` fset1 i;
-          }
-        }
-        r <- Some (k, c');
-      }
-      return r;
-    }
-
-    proc receive(i: int, c: pdh * sig, ch: bool): sskey option = {
-      var st_i, k, h, sig, b;
-      var ko <- None;
-
-      if (0 < i <= n /\ i \notin q) {
-        st_i <- oget c_map.[i];
-        q <- q `|` fset1 i;
-        
-        if (c \notin odflt fset0 r_map.[p_map.[i], i]) {
-          (h, sig) <- c;
-          b <@ S.verify(st_i.`pk, (st_i.`epk, h), sig);
-          if (b) {
-            k <@ RO.get(st_i.`epk, h, h ^ st_i.`esk);
-            ko <- Some k;
-          }
-          if (   ch
-              /\ i \notin xp
-              /\ p_map.[i] <> None /\ 0 < oget p_map.[i] <= m /\ oget p_map.[i] \notin cr
-              /\ ko <> None) {
-            bad_2 <- true;
-            ko <- None;
-            ich <- ich `|` fset1 i;
-          }
-        }
-      }
-      return ko;
-    }
-
-    proc h = RO.get
-  }
-
-  proc run(b) = {
-    var b';
-
-    RO.init();
-
-    b_ror <- b;
-
-    m <- 0;
-    n <- 0;
-
-    q <- fset0;
-    ich <- fset0;
-    rch <- fset0;
-    xp <- fset0;
-    cr <- fset0;
-
-    p_map <- empty;
-    i_map <- empty;
-    r_map <- empty;
-
-    pk_map <- empty;
-    sk_map <- empty;
-    c_map <- empty;
-
-    bad_1 <- false;
-    bad_2 <- false;
-
-    b' <@ A(Oracles).distinguish();
-    return b';
-  }
-}.
-
+(** Hop 2: Game 1 and Game 2 are equivalent unless (and until) the
+    adversary successfully triggers bad_2 in Game 2.
+**)
 local lemma Hop2 b &m:
   `|Pr[Game1_b.run(b) @ &m: res] - Pr[Game2_b.run(b) @ &m: res]|
   <= Pr[Game2_b.run(b) @ &m: Game1_b.bad_2].
 admitted.
+
+(** Reduction for Hop 2: If bad_2 happens, then we can extract a
+    forgery, regardless of the challenge bit.
+**)
+local lemma Reduction1 b &m:
+     B1.b_ror{m} = b
+  => Pr[Game2_b.run(b) @ &m: Game1_b.bad_2]
+     <= Pr[SUFCMA(S, B1(S, A)).run() @ &m: res].
+abort.
+
+(* We'd need to prove the same thing twice (once for each b) if we
+   prove it directly on probabilities. But we can be a bit more clever
+   by going one level down.
+*)
+local equiv Reduction1_equiv:
+  Game2_b.run ~ SUFCMA(S, B1(S, A)).run:
+       ={glob A, glob S, glob RO}
+    /\ b{1} = B1.b_ror{2}
+    ==> Game1_b.bad_2{1} => res{2}.
+(** HERE BE DRAGONS: we cannot immediately conclude that running
+    verification after the adversary returns (on the right) will
+    always give the same result as running it before the adversary's
+    run concludes (on the left). Here, we might just need to actually
+    halt and prevent the adversary to trigger more signing on the
+    left. (Or to restrict the class of signing algorithms the result
+    applies to, to a very reasonable class of algorithms where "if
+    verification succeeds once, then it succeeds every time on the
+    same input". This is slightly less reasonable if we want to allow
+    for stateful signature schemes...
+**)
+admitted.
+
+local lemma Reduction1_0 &m:
+  Pr[Game2_b.run(false) @ &m: Game1_b.bad_2]
+  <= Pr[SUFCMA(S, B1_0(S, A)).run() @ &m: res].
+proof.
+byequiv (: ={glob A, glob S, glob RO} /\ !b{1} ==> Game1_b.bad_2{1} => res{2})=> //.
+proc *.
+transitivity {2}
+  { B1.b_ror <- false;
+    r <@ SUFCMA(S, B1(S, A)).run(); }
+  (={glob A, glob S, glob RO} /\ !b{1} ==> Game1_b.bad_2{1} => r{2})
+  (={glob A, glob S, glob RO} ==> ={r})=> [/#|/>||].
++ by call Reduction1_equiv; auto=> />.
++ inline *; swap {2} 7 -6.
+  sim; wp=> />.
+  by sim: (={B1.forgery, b, SUFCMA.q, SUFCMA.cr, SUFCMA.pk_map, SUFCMA.n, glob S})=> />.
+qed.
+
+local lemma Reduction1_1 &m:
+  Pr[Game2_b.run(true) @ &m: Game1_b.bad_2]
+  <= Pr[SUFCMA(S, B1_1(S, A)).run() @ &m: res].
+proof.
+byequiv (: ={glob A, glob S, glob RO} /\ b{1} ==> Game1_b.bad_2{1} => res{2})=> //.
+proc *.
+transitivity {2}
+  { B1.b_ror <- true;
+    r <@ SUFCMA(S, B1(S, A)).run(); }
+  (={glob A, glob S, glob RO} /\ b{1} ==> Game1_b.bad_2{1} => r{2})
+  (={glob A, glob S, glob RO} ==> ={r})=> [/#|/>||].
++ by call Reduction1_equiv; auto=> />.
++ inline *; swap {2} 7 -6.
+  sim; wp=> />.
+  by sim: (={B1.forgery, b, SUFCMA.q, SUFCMA.cr, SUFCMA.pk_map, SUFCMA.n, glob S})=> />.
+qed.
 
 local module Game3_b = {
   include var Exp_b(SignedDH(S), RO, A) [-run]
@@ -1166,11 +1341,11 @@ local lemma Security_of_SignedDH &m:
     - Pr[Exp_b(SignedDH(S), RO, A).run(true) @ &m : res]|
   <=   Pr[Game1_b.run(true) @ &m: Game1_b.bad_1]
      + Pr[Game1_b.run(false) @ &m: Game1_b.bad_1]
-     + Pr[Game2_b.run(true) @ &m : Game1_b.bad_2]
-     + Pr[Game2_b.run(false) @ &m : Game1_b.bad_2]
+     + Pr[SUFCMA(S, B1_0(S, A)).run() @ &m: res]
+     + Pr[SUFCMA(S, B1_1(S, A)).run() @ &m: res]
      + 2%r * p
      + Pr[St_CDH(B2(S,A)).run() @ &m: res].
 proof.
-smt(Hop0 Hop1 Hop2 Hop3 Reduction).
+smt(Hop0 Hop1 Hop2 Reduction1_0 Reduction1_1 Hop3 Reduction).
 qed.
 end section.
